\documentclass[11pt]{article}
\usepackage[letterpaper, margin=1in]{geometry}
\usepackage{amsmath, amssymb, graphicx, epsfig, fleqn}
\setlength{\parindent}{0pt}
\newcommand{\ud}{\,\mathrm{d}}
\everymath{\displaystyle}
\def\FillInBlank{\rule{2.5in}{.01in} }
\pagestyle{empty}

\begin{document}
\begin{center}
\Large
\rm{Math 112}
\\
\rm{Chapter 11.6:  Root and Ratio Tests}
\\
\end{center}
\vspace{0.2in}
\fboxsep0.5cm

{\bf Ratio Test:}  \\

  \begin{displaymath}
\mbox{If} \lim_{n\to \infty}\left|\frac{a_{n+1}}{a_n}\right| = L < 1 \,, \mbox{then } \sum_1^{\infty}a_n \, \mbox{converges absolutely.}
  \end{displaymath}
    \begin{displaymath}
\mbox{If} \lim_{n\to \infty}\left|\frac{a_{n+1}}{a_n}\right| = L > 1 \,, \mbox{then } \sum_1^{\infty}a_n \, \mbox{diverges.}
      \end{displaymath}
  \begin{displaymath}
\mbox{If} \lim_{n\to \infty}\left|\frac{a_{n+1}}{a_n}\right| = 1 \,, \mbox{then the Ratio Test is inconclusive.}
      \end{displaymath}

  \vspace{0.2in}

 EXAMPLES:\\

 $\sum_{n=1}^{\infty} \frac{n^2}{5^n}$

 \vspace{1.5in}
 
 $\sum_{n=1}^{\infty} \frac{(-1)^{n-1}2^n}{n^n}$


 \vspace{1.5in}
 
 $\sum_{n=1}^{\infty} \frac{n^{10}8^n}{n!}$

 \pagebreak

  $\sum_{n=1}^{\infty} \frac{(-1)^{n+1}n}{\sqrt{n^3+2}}$


 \vspace{3in}

$\frac14 + \frac14\cdot\frac57 +  \frac14\cdot\frac57\cdot\frac{9}{10} + $


\vspace{2.5in}


$\sum_{n=2}^{\infty} \frac{(-1)^{n-1}}{n\ln{n}}$

\pagebreak

{\bf Root Test:}  \\

  \begin{displaymath}
\mbox{If} \lim_{n\to \infty}\sqrt[n]{|a_n|} = L < 1 \,, \mbox{then } \sum_1^{\infty}a_n \, \mbox{converges absolutely.}
  \end{displaymath}
    \begin{displaymath}
\mbox{If} \lim_{n\to \infty}\sqrt[n]{|a_n|} = L > 1 \,, \mbox{then } \sum_1^{\infty}a_n \, \mbox{diverges.}
      \end{displaymath}
  \begin{displaymath}
\mbox{If} \lim_{n\to \infty}\sqrt[n]{|a_n|} = 1 \,, \mbox{then the Root Test is inconclusive.}
      \end{displaymath}

  \vspace{0.2in}
  
  EXAMPLES:\\

  $\sum_{n=1}^{\infty} \frac{(-1)^{n-1}2^n}{n^n}$

  \vspace{2in}
  
    $\sum_{n=1}^{\infty} \left(\frac{3n}{2n+1}\right)^{4n}$  

\pagebreak

    $\sum_{n=1}^{\infty} \left(\frac{n}{\ln{n}}\right)^{2n}$  


\vspace{2in}

    $\sum_{n=1}^{\infty} \frac{(3n+1)^n}{n^{2n}}$  

\vspace{2in}

    $\sum_{n=1}^{\infty} \left(1 + \frac{1}{n}\right)^{n^2}$  

\end{document}




